code/experimental/P256/Hacl.Spec.ECDSAP256.Definition.fst
@@ -15,6 +15,23 @@ let prime_p256_order:pos =
   assert_norm (115792089210356248762697446949407573529996955224135760342422259061068512044369> 0);
   115792089210356248762697446949407573529996955224135760342422259061068512044369
 
+inline_for_extraction noextract
+let p256_order_prime_list : x:list uint64{List.Tot.length x == 4 /\ 
+  (
+    let open FStar.Mul in 
+    let l0 = uint_v (List.Tot.index x 0) in 
+    let l1 = uint_v (List.Tot.index x 1) in 
+    let l2 = uint_v (List.Tot.index x 2) in 
+    let l3 = uint_v (List.Tot.index x 3) in 
+    l0 + l1 * pow2 64 + l2 * pow2 128 + l3 * pow2 192 == prime_p256_order)
+  } =
+  let open FStar.Mul in 
+  [@inline_let]
+  let x =
+    [ (u64 17562291160714782033);  (u64 13611842547513532036); (u64 18446744073709551615);  (u64 18446744069414584320);] in
+    assert_norm(17562291160714782033 + 13611842547513532036 * pow2 64 + 18446744073709551615* pow2 128 + 18446744069414584320 * pow2 192 == prime_p256_order);
+  x  
+
 inline_for_extraction
 let felem = lbuffer uint64 (size 4)
 inline_for_extraction 
@@ -160,4 +177,16 @@ let felem_seq_as_nat_8 (a: lseq uint64 8) : Tot nat =
   uint_v a5 * pow2 64 * pow2 64 * pow2 64 * pow2 64 * pow2 64 + 
   uint_v a6 * pow2 64 * pow2 64 * pow2 64 * pow2 64 * pow2 64 * pow2 64 + 
   uint_v a7 * pow2 64 * pow2 64 * pow2 64 * pow2 64 * pow2 64 * pow2 64 * pow2 64
+
+noextract
+let felem_seq = lseq uint64 4
+
+noextract
+let felem_seq_as_nat (a: felem_seq) : Tot nat  = 
+  let open FStar.Mul in 
+  let a0 = Lib.Sequence.index a 0 in 
+  let a1 =  Lib.Sequence.index a 1 in 
+  let a2 =  Lib.Sequence.index  a 2 in 
+  let a3 =  Lib.Sequence.index a 3 in 
+  uint_v a0 + uint_v a1 * pow2 64 + uint_v a2 * pow2 64 * pow2 64 + uint_v a3 * pow2 64 * pow2 64 * pow2 64
 
